TM/Basic/Nop.v
@@ -30,7 +30,7 @@ Section Nop.
     intros ?. exists (initc nop input). cbn. firstorder.
   Qed.
 
-  Lemma Nop_sem: Nop ⊫ Nop_Rel.
+  Lemma Nop_sem: Nop ⊨ Nop_Rel.
   Proof.
     intros ? ? ? ?. hnf. destruct i; cbn in *; now inv H.
   Qed.
@@ -44,7 +44,7 @@ Arguments Nop_Rel {n sig F} (f) x y/.
 
 Ltac smpl_TM_Nop :=
   match goal with
-  | [ |- Nop _ _ _ ⊫ _] => eapply Nop_sem
+  | [ |- Nop _ _ _ ⊨ _] => eapply Nop_sem
   | [ |- Nop _ _ _ ⊨c(_) _] => eapply Nop_total
   | [ |- projT1 (Nop _ _ _) ↓ _] => eapply RealiseIn_terminatesIn, Nop_total
   end.
